Logic/Modal/Standard/Kripke/Preservation.lean
@@ -7,102 +7,116 @@ namespace Kripke
 
 section Bisimulation
 
-
 end Bisimulation
 
 
 section Generation
 
+/-
 class GeneratedSubframe (F F' : Kripke.Frame α) where
   subset : F'.World ⊆ F.World
   rel : ∀ {x y : F'.World}, x ≺ y ↔ F.Rel' ⟨x, (by aesop)⟩ ⟨y, (by aesop)⟩ -- MEMO: i.e. F.Rel' = F.Rel' ∪ (F.World × F.World)
   closed : ∀ {x : F'.World}, ∀ {y : F.World}, ⟨x.1, (by aesop)⟩ ≺ y → y.1 ∈ F'.World
-
+-/
 
 end Generation
 
+section pMorphism
 
-section Reduction
+variable {α δ₁ δ₂}
 
-protected class Frame.reduction {F₁ F₂ : Kripke.Frame α} (f : F₁.World → F₂.World)  where
-  forth : ∀ {w v : F₁.World}, w ≺ v → (f w) ≺ (f v)
-  back : ∀ {w : F₁.World}, ∀ {v : F₂.World}, (f w) ≺ v → ∃ u, w ≺ u ∧ f u = v
+structure Frame.pMorphism (F₁ : Kripke.Frame δ₁) (F₂ : Kripke.Frame δ₂) where
+  toFun : F₁.World → F₂.World
+  forth {x y : F₁.World} : x ≺ y → toFun x ≺ toFun y
+  back {w : F₁.World} {v : F₂.World} : toFun w ≺ v → ∃ u, w ≺ u ∧ toFun u = v
+
+infix:80 " →ₚ " => Frame.pMorphism
+
+instance : CoeFun (Frame.pMorphism F₁ F₂) (λ _ => F₁.World → F₂.World) := ⟨λ f => f.toFun⟩
 
 
-protected class Model.reduction {M₁ M₂ : Kripke.Model δ α} (f : M₁.World → M₂.World)  extends Frame.reduction f where
-  atomic : ∀ {w : M₁.World}, ∀ {a}, (M₁.Valuation w a) ↔ (M₂.Valuation (f w) a)
+structure Model.pMorphism (M₁ : Kripke.Model δ₁ α) (M₂ : Kripke.Model δ₂ α) extends M₁.Frame →ₚ M₂.Frame where
+  atomic {w : M₁.World} {a} : (M₁.Valuation w a) ↔ (M₂.Valuation (toFun w) a)
+
+infix:80 " →ₚ " => Model.pMorphism
+
+instance : CoeFun (Model.pMorphism M₁ M₂) (λ _ => M₁.World → M₂.World) := ⟨λ f => f.toFun⟩
 
 
 open Formula
 
-variable {F₁ F₂ : Kripke.Frame' δ α} {M₁ M₂ : Kripke.Model δ α} {p : Formula α}
+variable {F₁ : Kripke.Frame δ₁} {F₂ : Kripke.Frame δ₂}
+         {M₁ : Kripke.Model δ₁ α} {M₂ : Kripke.Model δ₂ α}
+         {p : Formula α}
 
-lemma iff_formula_satisfies_morphism (f : M₁.World → M₂.World) [Model.reduction f] {w : M₁.World}
-  : (⟨M₁, w⟩ : (M : Model δ α) × M.World) ⊧ p ↔ (⟨M₂, (f w)⟩ : (M : Model δ α) × M.World) ⊧ p := by
+lemma iff_formula_satisfies_morphism (f : M₁ →ₚ M₂) {w : M₁.World}
+  : w ⊧ p ↔ (f w) ⊧ p := by
   induction p using Formula.rec' generalizing w with
   | hatom p =>
     constructor;
-    . apply Model.reduction.atomic |>.mp;
-    . apply Model.reduction.atomic |>.mpr
+    . apply f.atomic |>.mp;
+    . apply f.atomic |>.mpr
   | hbox p ih =>
     constructor;
     . intro h w₂ hw₂;
-      obtain ⟨w₁, ⟨hww₁, e⟩⟩ := Frame.reduction.back hw₂;
-      have := ih.mp $ h hww₁;
-      subst e;
-      assumption;
+      obtain ⟨w₁, hww₁, e⟩ := f.back hw₂; subst e;
+      exact ih.mp $ h hww₁;
     . intro h w' hww';
-      exact ih.mpr $ h $ Frame.reduction.forth hww';
+      exact ih.mpr $ h $ f.forth hww';
   | _ => simp_all [kripke_satisfies];
 
-lemma iff_formula_valid_on_frame_surjective_morphism (f : F₁.World → F₂.World) [Frame.reduction f] (f_surjective : f.Surjective) : F₁ ⊧ p → F₂ ⊧ p := by
+lemma iff_formula_valid_on_frame_surjective_morphism (f : F₁ →ₚ F₂) (f_surjective : Function.Surjective f) : F₁[α] ⊧ p → F₂[α] ⊧ p := by
   contrapose;
   intro h;
-  obtain ⟨V₂, w₂, hw₂, h⟩ := by simpa [valid_on_KripkeFrame, valid_on_KripkeModel] using h;
+  obtain ⟨V₂, w₂, h⟩ := by simpa [valid_on_KripkeFrame, valid_on_KripkeModel] using h;
   simp [valid_on_KripkeFrame, valid_on_KripkeModel];
 
-  obtain ⟨w₁, e⟩ := f_surjective ⟨w₂, hw₂⟩; rw [←e] at h;
+  obtain ⟨w₁, e⟩ := f_surjective w₂; subst e;
   let V₁ := λ w a => V₂ (f w) a;
-  use V₁, w₁.1, w₁.2;
+  use V₁, w₁;
 
-  let M₁ : Model δ α := { Frame := F₁, Valuation := V₁ };
-  let M₂ : Model δ α := { Frame := F₂, Valuation := V₂ };
-  have : Model.reduction (M₁ := M₁) (M₂ := M₂) f := { atomic := by simp_all };
-  exact iff_formula_satisfies_morphism (M₁ := M₁) (M₂ := M₂) f |>.not.mpr h;
+  let M₁ : Model δ₁ α := { Frame := F₁, Valuation := V₁ };
+  let M₂ : Model δ₂ α := { Frame := F₂, Valuation := V₂ };
+  exact iff_formula_satisfies_morphism (M₁ := M₁) (M₂ := M₂) {
+    toFun := f,
+    forth := f.forth,
+    back := f.back,
+    atomic := by simp_all
+  } |>.not.mpr h;
 
-lemma iff_theory_valid_on_frame_surjective_morphism (f : F₁.World → F₂.World) [Frame.reduction f] (f_surjective : f.Surjective) : F₁ ⊧* T → F₂ ⊧* T := by
+lemma iff_theory_valid_on_frame_surjective_morphism (f : F₁ →ₚ F₂) (f_surjective : Function.Surjective f) : F₁[α] ⊧* T → F₂[α] ⊧* T := by
   simp only [Semantics.realizeSet_iff];
   intro h p hp;
   exact iff_formula_valid_on_frame_surjective_morphism f f_surjective (h hp);
 
 abbrev IrreflexiveFrameClass : FrameClass := λ ⟨_, F⟩ => Irreflexive F
 
-theorem undefinable_irreflexive : ¬∃ (Ax : AxiomSet α), Ax.DefinesKripkeFrameClass IrreflexiveFrameClass := by
+theorem undefinable_irreflexive : ¬∃ (Ax : AxiomSet α), AxiomSet.DefinesKripkeFrameClass.{_, 0} Ax IrreflexiveFrameClass := by
   by_contra hC;
   obtain ⟨Ax, h⟩ := hC;
 
-  -- MEMO: `Rel := { (x, y) | x ≠ y }`で行けてほしいのだがなぜか通らない．
-  let F₁ : Frame' (Fin 2) α := { World := {0, 1}, Rel := {(⟨0, by simp⟩, ⟨1, by simp⟩), (⟨1, by simp⟩, ⟨0, by simp⟩)} };
+  let F₁ : Frame (Fin 2) := { Rel := (· ≠ ·) };
   have hIF₁ : Irreflexive F₁ := by simp [Irreflexive, Frame.Rel'];
 
-  let F₂ : Frame' (Fin 2) α := { World := {0}, Rel := { (x, y) | x = y } };
-  have hIF₂ : ¬Irreflexive F₂ := by simp [Irreflexive]; use ⟨0, (by simp)⟩; simp [Frame.Rel'];
+  let F₂ : Frame (Fin 1) := { Rel := (· = ·) };
 
-  let f : F₁.World → F₂.World := λ _ => ⟨0, (by simp)⟩;
-  have hSur : Function.Surjective f := by simp [Function.Surjective]; aesop;
-  have : Frame.reduction f := {
-    forth := by simp [Frame.Rel'];
+  let f : F₁ →ₚ F₂ := {
+    toFun := λ _ => 0,
+    forth := by simp [Frame.Rel'],
     back := by
-      intro x y Rxy; simp [Frame.Rel'] at Rxy;
-      match x with
-      | ⟨0, _⟩ => use ⟨1, (by simp)⟩; simp_all [Frame.Rel'];
-      | ⟨1, _⟩ => use ⟨0, (by simp)⟩; simp_all [Frame.Rel'];
+      simp;
+      intro w;
+      match w with
+      | 0 => use 1; simp [Frame.Rel'];
+      | 1 => use 0; simp [Frame.Rel'];
   };
-  have : Irreflexive F₂ := h.mp $ iff_theory_valid_on_frame_surjective_morphism f hSur $ h.mpr hIF₁;
+  have f_surjective : Function.Surjective f := by simp [Function.Surjective]; aesop;
+
+  have : ¬Irreflexive F₂ := by simp [Irreflexive];
+  have : Irreflexive F₂ := h.mp $ iff_theory_valid_on_frame_surjective_morphism f f_surjective $ h.mpr hIF₁;
   contradiction;
 
-end Reduction
-
+end pMorphism
 
 end Kripke
 
