Logic/Modal/Standard/Kripke/Soundness.lean
@@ -3,12 +3,15 @@ import Logic.Modal.Standard.Deduction
 
 namespace LO.Modal.Standard.Kripke
 
-variable {Ax : AxiomSet α} {𝔽 : FrameClass}
+variable {Ax : AxiomSet α}
 
-open Deduction
 open Formula
-
+open Deduction
 open DeductionParameter (Normal)
+
+section
+
+variable {𝔽 : FrameClass}
 
 lemma sound (defines : Ax.DefinesKripkeFrameClass 𝔽) (d : Axᴺ ⊢! p) : 𝔽[α] ⊧ p := by
   induction d using Deduction.inducition_with_necOnly! with
@@ -30,34 +33,36 @@ lemma sound (defines : Ax.DefinesKripkeFrameClass 𝔽) (d : Axᴺ ⊢! p) : �
 
 lemma sound_of_defines (defines : Ax.DefinesKripkeFrameClass 𝔽) : Sound Axᴺ 𝔽[α] := ⟨sound defines⟩
 
-instance K_sound : Sound 𝐊 AllFrameClass[α] := by simpa [←Normal.isK] using sound_of_defines axiomK_defines;
-
-
 lemma unprovable_bot_of_nonempty_frameClass (defines : Ax.DefinesKripkeFrameClass 𝔽) (nonempty : 𝔽.Nonempty) : Axᴺ ⊬! ⊥ := by
   by_contra hC;
-  obtain ⟨⟨α, F⟩, hF⟩ := nonempty;
+  obtain ⟨⟨_, F⟩, hF⟩ := nonempty;
   simpa using sound defines hC hF;
 
 lemma consistent_of_defines (defines : Ax.DefinesKripkeFrameClass 𝔽) (nonempty : 𝔽.Nonempty) : System.Consistent Axᴺ := by
   apply System.Consistent.of_unprovable;
   exact unprovable_bot_of_nonempty_frameClass defines nonempty;
 
+instance K_sound : Sound 𝐊 AllFrameClass[α] := by simpa [←Normal.isK] using sound_of_defines axiomK_defines;
+
 instance K_consistent' : System.Consistent (𝗞 : AxiomSet α)ᴺ := consistent_of_defines axiomK_defines AllFrameClass.nonempty
 
 instance K_consistent : System.Consistent (𝐊 : DeductionParameter α) := by
   simpa [←Normal.isK] using K_consistent';
 
+end
 
-/-
-lemma finite_sound (defines : Ax.FinitelyDefinesKripkeFrameClass 𝔽) (d : Axᴺ ⊢! p) : 𝔽ᶠ ⊧ p := by
+section
+
+variable {𝔽 : FiniteFrameClass}
+
+lemma finite_sound (defines : Ax.FinitelyDefinesKripkeFrameClass 𝔽) (d : Axᴺ ⊢! p) : (𝔽 : FrameClass)[α] ⊧ p := by
   induction d using Deduction.inducition_with_necOnly! with
   | hMaxm h =>
     simp only [Set.mem_setOf_eq] at h;
     rcases h with (hK | hR);
     . exact (Semantics.RealizeSet.setOf_iff.mp valid_on_KripkeFrameClass.axiomK) _ hK;
-    . intro F hF;
-      simp [FrameClass.toFinite] at hF;
-      apply Semantics.RealizeSet.setOf_iff.mp (defines hF.2 |>.mpr hF.1) _ hR;
+    . rintro δ F ⟨FF, hFF, eFF⟩; subst eFF;
+      exact Semantics.RealizeSet.setOf_iff.mp (defines.mpr hFF) _ hR;
   | hMdp ihpq ihp => exact valid_on_KripkeFrameClass.mdp ihpq ihp;
   | hNec ih => exact valid_on_KripkeFrameClass.nec ih;
   | hDisj₃ =>
@@ -68,16 +73,20 @@ lemma finite_sound (defines : Ax.FinitelyDefinesKripkeFrameClass 𝔽) (d : Ax�
     | inr hq => exact hqr hq;
   | _ => simp_all [valid_on_KripkeFrameClass, valid_on_KripkeFrame, valid_on_KripkeModel, kripke_satisfies];
 
-lemma sound_of_finitely_defines (defines : Ax.FinitelyDefinesKripkeFrameClass 𝔽) : Sound Axᴺ 𝔽ᶠ := ⟨finite_sound defines⟩
+lemma sound_of_finitely_defines (defines : Ax.FinitelyDefinesKripkeFrameClass 𝔽) : Sound Axᴺ ↑𝔽[α] := ⟨finite_sound defines⟩
 
-lemma unprovable_bot_of_nonempty_finite_frameClass (defines : Ax.FinitelyDefinesKripkeFrameClass 𝔽) (nonempty : 𝔽ᶠ.Nonempty) : Axᴺ ⊬! ⊥ := by
+lemma unprovable_bot_of_nonempty_finite_frameClass (defines : Ax.FinitelyDefinesKripkeFrameClass 𝔽) (nonempty : 𝔽.Nonempty) : Axᴺ ⊬! ⊥ := by
   by_contra hC;
-  obtain ⟨F, hF⟩ := nonempty;
-  simpa using finite_sound defines hC F hF;
+  obtain ⟨⟨δ, F⟩, hF⟩ := nonempty;
+  have := @finite_sound α Ax 𝔽 ⊥ defines hC δ ↑F;
+  simp [FiniteFrameClass.toFrameClass] at this;
+  have := this F hF;
+  contradiction;
 
-lemma consistent_of_finitely_defines (defines : Ax.FinitelyDefinesKripkeFrameClass 𝔽) (nonempty : 𝔽ᶠ.Nonempty) : System.Consistent Axᴺ := by
+lemma consistent_of_finitely_defines (defines : Ax.FinitelyDefinesKripkeFrameClass 𝔽) (nonempty : 𝔽.Nonempty) : System.Consistent Axᴺ := by
   apply System.Consistent.of_unprovable;
   exact unprovable_bot_of_nonempty_finite_frameClass defines nonempty;
--/
+
+end
 
 end LO.Modal.Standard.Kripke
